% Created 2015-05-12 Tue 22:37
\documentclass[a4paper]{article}
\usepackage[utf8]{inputenc}
\usepackage[T1]{fontenc}
\usepackage{fixltx2e}
\usepackage{graphicx}
\usepackage{longtable}
\usepackage{float}
\usepackage{wrapfig}
\usepackage{rotating}
\usepackage[normalem]{ulem}
\usepackage{amsmath}
\usepackage{textcomp}
\usepackage{marvosym}
\usepackage{wasysym}
\usepackage{amssymb}
\usepackage{hyperref}
\tolerance=1000
\usepackage[utf8]{inputenc}
\usepackage[usenames,dvipsnames]{color}
\usepackage{commath}
\usepackage{tikz}
\usetikzlibrary{shapes,backgrounds}
\usepackage{marginnote}
\usepackage{listings}
\usepackage{color}
\usepackage{enumerate}
\hypersetup{urlcolor=blue}
\hypersetup{colorlinks,urlcolor=blue}
\setlength{\parskip}{16pt plus 2pt minus 2pt}
\definecolor{codebg}{rgb}{0.96,0.99,0.8}
\definecolor{codestr}{rgb}{0.46,0.09,0.2}
\DeclareMathOperator{\Dom}{Dom}
\allowdisplaybreaks[4]
\author{Oleg Sivokon}
\date{\textit{<2015-04-03 Fri>}}
\title{Assignment 14, Infinitesimal Calculus}
\hypersetup{
  pdfkeywords={Infinitesimal Calculus, Assignment, Limits of functions},
  pdfsubject={Fourth asssignment in the course Infinitesimal Calculus},
  pdfcreator={Emacs 25.0.50.1 (Org mode 8.2.2)}}
\begin{document}

\maketitle
\tableofcontents


\definecolor{codebg}{rgb}{0.96,0.99,0.8}
\lstnewenvironment{maxima}{%
  \lstset{backgroundcolor=\color{codebg},
    aboveskip=20pt,
    showstringspaces=false,
    frame=single,
    framerule=0pt,
    basicstyle=\ttfamily\scriptsize,
    columns=fixed}}{}
}
\makeatletter
\newcommand{\verbatimfont}[1]{\renewcommand{\verbatim@font}{\ttfamily#1}}
\makeatother
\verbatimfont{\small}%
\clearpage

\section{Problems}
\label{sec-1}

\subsection{Problem 1}
\label{sec-1-1}
\begin{enumerate}
\item Find the domain of $f$ defined as $f(x) = \sqrt{\tan x - 1}$.
\item Find all values of $x$ in segment $[0, \pi]$, for which $\abs{\tan x} \leq \sin 2x}$.
\end{enumerate}

\subsubsection{Answer 1}
\label{sec-1-1-1}
$\tan x > 1$ where $\frac{\pi}{4} < x \bmod \frac{\pi}{2} < \frac{\pi}{2}$.
Since we assume that $f$ is real-valued, we cannot extract roots from negative numbers.

Hence $\Dom(f) = \{x \in \mathbb{R} \; | \; \frac{\pi}{4} < x \bmod \frac{\pi}{2}
    < \frac{\pi}{2}\}$.

\begin{maxima}
programmode: false;
print (plot2d (tan(x),
    [x, -2 * %pi, 2 * %pi], [y, -3, 3],
    [gnuplot_pdf_term_command, 
     "set term cairolatex standalone pdf size 16cm,10.5cm"],
    [gnuplot_postamble,
     "set arrow from pi/4,-3 to pi/4,3 nohead
      set arrow from pi*5/4,-3 to pi*5/4,3 nohead
      set arrow from -2*pi,1 to 2*pi,1 nohead"],
    [ytics, 1, 1, 1], [xtics, 0, 1, 0],
    [label, ["${\\displaystyle \\frac{\\pi}{4}}$", 1.4, 2.4],
            ["${\\displaystyle \\frac{5\\pi}{4}}$", 3.2, 2.4]],
    [title, "Tangent curve"], [pdf_file, %out]));
\end{maxima}

\includegraphics[width=0.9\textwidth]{/home/wvxvw/Documents/uni/infinitesimal-calculus/tangent_x.pdf}
\subsubsection{Answer 2}
\label{sec-1-1-2}
Both functions attain the same values at 0 and $\frac{\pi}{4}$.  But sine is
a concave function and tanget is a convex function, thus tangent must be less
than sine at this interval.  Tangent keeps increasing until $\frac{\pi}{2}$,
while sine will be decreasing until $\frac{3\pi}{2}$, thus, on this interval
tangent is greater than sine.  The functions meet again at $x=\pi$.

\begin{maxima}
programmode: false;
gnuplot_pdf_command: %command;
print(plot2d ([abs(tan(x)), sin(2 * x)],
    [x, -2 * %pi, 2 * %pi], [y, -1.5, 3],
    [gnuplot_pdf_term_command, 
     "set term cairolatex standalone pdf size 16cm,10.5cm"],
    [gnuplot_postamble,
     "set arrow from pi/4,-1.5 to pi/4,3 nohead
      set arrow from pi,-1.5 to pi,3 nohead
      set arrow from -2*pi,1 to 2*pi,1 nohead
      set key spacing 1.8 left bottom"],
    [xtics, 0, 1, 0], [ytics, 1, 1, 1],
    [label, ["${\\displaystyle \\frac{\\pi}{4}}$", 1.4, 2.1],
            ["${\\displaystyle \\pi}$", 3.4, 2.1]],
    [title, "Tangent curve intersecting with sine curve"],
    [pdf_file, %out]));
\end{maxima}

\includegraphics[width=0.9\textwidth]{/home/wvxvw/Documents/uni/infinitesimal-calculus/abstangent_x.pdf}
\subsection{Problem 2}
\label{sec-1-2}
Let $f$, $g$ and $h$ be functions from $\mathbb{R}$ to $\mathbb{R}$.
\begin{enumerate}
\item If $f \circ g = f \circ h$, does it follow $g = h$?
\item If $f \circ g = f \circ h$, and $f$ is one-to-one, does it follow $g = h$?
\item If $f \circ g = f \circ h$, and $f$ is onto, does it follow $g = h$?
\item If $f \circ g$ is increasing, and $f$ is decreasing, does it follow that
      $g$ is increasing?
\item If $f \circ g$ is increasing, and $f$ is one-to-one, does it follow that
      $g$ is monotonic?
\end{enumerate}

\subsubsection{Answer 3}
\label{sec-1-2-1}
No, $g$ and $h$ are not necessarily equal.  Whenever co-domain of $f$
doesn't contain some real number, $g$ and $h$ may differ in that input.
For example, let $f(x) = 2x$, $g(x) = (x \bmod 2) + x$ and
$h(x) = (x \bmod 2) * 2 + x$.  Because $f$ in this example will only
generate even numbers, the $(x \bmod 2)$ term will always be zero,
thus $f \circ g = f \circ h$, but, obviously, $g \neq h$.
\subsubsection{Answer 4}
\label{sec-1-2-2}
No, it isn't sufficient for $f$ to be one-to-one to ensure right-cancellation
property under composition.  The example given in \ref{sec-1-2-1} is applicable
in this case too since whenever $f(x) = f(y)$ so is $x = y$ (since multiplication
does have the cancellation property).
\subsubsection{Answer 5}
\label{sec-1-2-3}
Yes, if $f$ is onto, then the composition is right-cancellable.  Suppose,
for contradiction it wasn't, then for some $y$ $g(y) \neq h(y)$, but
$y = f(x)$ (since by definition of a total function, every element in
its co-domain has an element in its domain).  Hence $g(f(x)) \neq h(f(x))$,
but we are given that $g \circ f = h \circ f$, which is a contradiction.
Hence functions are equal.
\subsubsection{Answer 6}
\label{sec-1-2-4}
No, $g$ doesn't need to be increasing.  Put $g(x) = f(x) = -x$, both $f$
and $g$ are decreasing but $f \circ g = Id$, which is an increasing function.
\subsubsection{Anser 7}
\label{sec-1-2-5}
No, $g$ is not necessarily monotonic.  Put $f(x) = x(-1)^x$ and $g(x) = \abs{x}$.
Then $(f \circ g)(x) = \abs{x(-1)^x} = x\abs{(-1)^x} = x$.  $f \circ g$ is
increasing, $f$ is one-to-one, but $g$ isn't monotonic: it decreases whenever
$x$ is negative and increases whenever $x$ is positive.
\subsection{Problem 3}
\label{sec-1-3}
\begin{enumerate}
\item Prove from $\epsilon-\delta$ definition of limit that 
      $\lim_{x \to 2}\sqrt{3x - 2} = 2$.
\item Prove from $\epsilon-M$ definition of limit that 
      $\lim_{x \to \infty}\frac{x}{x+\sin x} = 1$.
\end{enumerate}

\subsubsection{Answer 8}
\label{sec-1-3-1}
Recall the definition:
\begin{quote}
For all $\epsilon > 0$ there exists $\sigma > 0$ s.t. for all $x$ in
$\Dom(f(x))$ which satisfy $0 < \abs{x - x_0} < \sigma$ the inequality
$\abs{f(x) - L} < \epsilon$ holds.
\end{quote}

Let $\epsilon$ be arbitrary real, put
\begin{equation*}
  \begin{aligned}
      &\abs{f(x) - L}          &< \epsilon                         &\iff \\
      &\abs{\sqrt{3x - 2} - 2} &< \epsilon                               \\
      &\textit{Suppose $\sqrt{3x - 2} - 2 > 0$}                          \\
    0 &< \sqrt{3x - 2} - 2     &< \epsilon                         &\iff \\
    0 &< \sqrt{3x - 2}         &< \epsilon + 2                     &\iff \\
    0 &< 3x - 2                &< (\epsilon + 2)^2                 &\iff \\
    0 &< 3x - 2                &< \epsilon^2 + 4\epsilon + 4       &\iff \\
    0 &< 3x - 6                &< \epsilon^2 + 4\epsilon           &\iff \\
    0 &< x - 2                 &< \frac{\epsilon^2 + 4\epsilon}{3}       \\
      &\textit{Similarly for $\sqrt{3x - 2} - 2 < 0$}                    \\
    0 &> \sqrt{3x - 2} - 2     &> -\epsilon                        &\iff \\
    0 &> \sqrt{3x - 2}         &> -\epsilon + 2                    &\iff \\
    0 &> 3x - 2                &> (-\epsilon + 2)^2                &\iff \\
    0 &> 3x - 2                &> \epsilon^2 - 4\epsilon + 4       &\iff \\
    0 &> 3x - 6                &> \epsilon^2 - 4\epsilon           &\iff \\
    0 &> x - 2                 &> \frac{\epsilon^2 - 4\epsilon}{3}
  \end{aligned}
\end{equation*}

Hence, we can choose $\delta$ to be $\frac{\epsilon^2 - 4\epsilon}{3}$
whenever $x < x_0$ and $\frac{\epsilon^2 + 4\epsilon}{3}$ whenever
$x > x_0$, which completes the proof.
\subsubsection{Answer 9}
\label{sec-1-3-2}
Recall the definition:
\begin{quote}
For all $\epsilon > 0$ there exists $M > 0$ s.t. for all $x$ in
$\Dom(f(x))$ $x > M$ implies $\abs{f(x) - L} < \epsilon$.
\end{quote}

Let $\epsilon > 0$, then look for appropriate value for $x$:
\begin{align*}
  &\abs{\frac{x}{x + \sin x} - 1}                   &< \epsilon &\iff \\
  &\abs{\frac{x}{x + \sin x} - \sin^2 x - \cos^2 x} &< \epsilon &\iff \\
  &\abs{\frac{x - \sin^2 x(x + \sin x) -
      \cos^2 x(x + \sin x)}{x + \sin x}}            &< \epsilon &\iff \\
  &\abs{\frac{x - x\sin^2 x - \sin^3 x -
      x\cos^2 x - \cos^2 x \sin x}{x + \sin x}}     &< \epsilon &\iff \\
  &\abs{\frac{x(1 - \sin^2 - \cos^2 x) -
      \sin x(\sin^2 x - \cos^2)}{x + \sin x}}       &< \epsilon &\iff \\
  &\abs{\frac{x(1 - 1) - \sin x(1)}{x + \sin x}}    &< \epsilon &\iff \\
  &\abs{\frac{-\sin x}{x + \sin x}}                 &< \epsilon \\
\end{align*}

Assume $x > 0$:
\begin{align*}
  &\frac{-\sin x}{x + \sin x} &< \epsilon &\iff \\
  &-\sin x                    &< \epsilon(x + \sin x) &\iff \\
  &-\sin x                    &< \epsilon x + \epsilon \sin x &\iff \\
  &-\epsilon x                &< \sin x + \epsilon \sin x &\iff \\
  &-x                         &< \frac{\sin x + \epsilon \sin x}{\epsilon} &\iff \\
  &x                          &> \frac{\sin x(1 + \epsilon)}{\epsilon}
\end{align*}

Put $M = \max\left(0, \frac{\sin x(1 + \epsilon)}{\epsilon}\right)$. If $x > M$, then
$x > 0$ and $x > \frac{\sin x(1 + \epsilon)}{\epsilon}$, hence:
\begin{align*}
  &x                              &> \frac{\sin x(1 + \epsilon)}{\epsilon} \\
  &\hdots \textit{Reverse the calculations above} \\
  &\frac{-\sin x}{x + \sin x}     &< \epsilon \\
  &\hdots \\
  &\abs{\frac{x}{x + \sin x} - 1} &< \epsilon.
\end{align*}

Which completes the proof.
\subsection{Problem 4}
\label{sec-1-4}
\begin{enumerate}
\item Let $f$ be a function defined in the neighborhood of $x_0$.
Express ``$f$ doesn't have a limit at $x_0$'' using:
\begin{itemize}
\item $\epsilon-\sigma$ language.
\item Using Heine definition of limit (for sequences).
\end{itemize}

\item Prove that $f(x) = \frac{x}{x - \lfloor x \rfloor}$ doesn't have
a finite limit at $x \to 0$ in the following ways:
\begin{itemize}
\item By using $\epsilon-\sigma$ definition given above.
\item By using Heine definition of limit (also given above).
\end{itemize}
\end{enumerate}

\subsubsection{Answer 10}
\label{sec-1-4-1}

\subsubsection{Answer 11}
\label{sec-1-4-2}
\subsection{Problem 5}
\label{sec-1-5}
Find limits of:
\begin{enumerate}
\item $\lim_{x \to 0}\frac{1 - \cos x}{x \sin x}$.
\item $\lim_{x \to 0}\frac{x + 7x^3}{x^3 - 2x^4}$.
\item $\lim_{x \to 0}\frac{x^2 - 1}{2x^3 - x^2 - x}$.
\item $\lim_{x \to 0}(\sqrt{1 + x + x^2} - \sqrt{1 - x + x^2})$.
\item $\lim_{x \to k}\lfloor x \rfloor \tan \frac{\pi x}{2}$, $k = 0, 1, 2$.
\end{enumerate}

\subsubsection{Answer 12}
\label{sec-1-5-1}
\begin{maxima}
tex(limit((1 - cos(x)) / (x * sin(x)), x, 0));
\end{maxima}

$${{1}\over{2}}$$

\textbf{Proof:}
\begin{align*}
  \lim_{x \to 0}\frac{1 - \cos x}{x \sin x} &= 
  \lim_{x \to 0}\frac{(1 - \cos x) * (1 + \cos x)}{x \sin x (1 + \cos x)} \\
  &= \lim_{x \to 0}\frac{1 - \cos^2 x}{x \sin x (1 + \cos x)} \\
  &= \lim_{x \to 0}\frac{\sin^2 x}{x \sin x (1 + \cos x)} \\
  &= \lim_{x \to 0}\frac{\sin x}{x (1 + \cos x)} \\
  &= \lim_{x \to 0}\frac{\sin x}{x} * \lim_{x \to 0}\frac{1}{1 + \cos x} \\
  &= 1 * \lim_{x \to 0}\frac{1}{1 + \cos x} \\
  &= \lim_{x \to 0}\frac{1}{1 + 1} \\
  &= \frac{1}{2}
\end{align*}
\subsubsection{Answer 13}
\label{sec-1-5-2}
\begin{maxima}
tex(limit((x + 7 * x^3) / (x^3 - 2 * x^4), x, 0));
\end{maxima}

$$\infty $$

\textbf{Proof:}
\begin{align*}
  \lim_{x \to 0}\frac{x + 7x^3}{x^3 - 2x^4} &= 
  \lim_{x \to 0}\frac{1 + 7x^2}{x^2 - 2x^3} \\
  &= \lim_{x \to 0}\frac{1 - 4x^2}{x^2 - 2x^3} + \frac{11x^2}{x^2 - 2x^3} \\
  &= \lim_{x \to 0}\frac{(1 - 2x)(1 + 2x)}{x^2(1 - 2x)} + \frac{11}{1 + 2x} \\
  &= \lim_{x \to 0}\frac{1 + 2x}{x^2} + \frac{11}{1 + 2x} \\
  &= \lim_{x \to 0}\frac{1}{x^2} + \frac{2x}{x^2} + \frac{11}{1 + 2x} \\
  &= \lim_{x \to 0}\frac{1}{x^2} + \frac{2}{x} + \frac{11}{1 + 2x} \\
  &= \lim_{x \to 0}\frac{1}{x^2} + \lim_{x \to 0}\frac{2}{x} + \lim_{x \to 0}\frac{11}{1 + 2x} \\
  &= \infty + \infty + 11 & \textit{Using ifinite limits addition} \\
  &= \infty
\end{align*}
\subsubsection{Answer 14}
\label{sec-1-5-3}
\begin{maxima}
tex(limit((x^2 - 1) / (2 * x^3 - x^2 - x), x, 0));
\end{maxima}

$${\it infinity}$$

\textbf{Proof:}
\begin{align*}
  \lim_{x \to 0}\frac{x^2 - 1}{2x^3 - x^2 - x} &=
  \lim_{x \to 0}\frac{(x - 1)(x + 1)}{x^2(x - 1) + x(x^2 - 1)} \\
  &= \lim_{x \to 0}\frac{(x - 1)(x + 1)}{x^2(x - 1) + x(x - 1)(x + 1)} \\
  &= \lim_{x \to 0}\frac{(x - 1)(x + 1)}{(x - 1)(x^2 + x(x + 1))} \\
  &= \lim_{x \to 0}\frac{x + 1}{x^2 + x(x + 1)} \\
  &= \lim_{x \to 0}\frac{x + 1}{x^2 + x^2 + x} \\
  &= \lim_{x \to 0}\frac{x + 1}{2x^2 + x} \\
  &= \lim_{x \to 0}\frac{x + 1}{x(2x + 1)} \\
  &= \lim_{x \to 0}\frac{x + 1}{x} * \lim_{x \to 0}\frac{1}{2x + 1} \\
  &= \lim_{x \to 0}\frac{x + 1}{x} * 1 \\
  &= \infty
\end{align*}
\subsubsection{Answer 15}
\label{sec-1-5-4}
\begin{maxima}
tex(limit(sqrt(1 + x + x^2) - sqrt(1 - x + x^2), x, 0));
\end{maxima}

$$0$$

\textbf{Proof:} this function is continuous at $x = 0$ since square root
is continuous at 1 and this function is offset by one.  From definition
of continuity we know that the limit of the function coincides with its
value, hence the limit is $\sqrt{1 + 0 + 0^2} - \sqrt{1 - 0 + 0^2} = 1 - 1 = 0$.
\subsubsection{Answer 16}
\label{sec-1-5-5}
\begin{maxima}
for i : 0 thru 2 do
    tex(limit(floor(x) * tan((%pi * x) / 2), x, i));
\end{maxima}

$$0$$
$${\it und}$$
$$0$$
% Emacs 25.0.50.1 (Org mode 8.2.2)
\end{document}